Challenge/Modexp/Submission/Proofs/Fast/Paths/P0.lean
@@ -54,10 +54,14 @@ def blk1003 :
    opAt 449 .ADD,
    opAt 450 (.Dup ⟨0, by decide⟩),
    opAt 451 .CALLDATALOAD,
-   pushAt 452 5 255,
+   pushAt 452 1 255,
    opAt 453 .SHR,
-   opAt 454 .ISZERO,
-   pushAt 455 2 800,
-   opAt 456 .JUMPI]
+   opAt 454 .JUMPDEST,
+   opAt 455 .JUMPDEST,
+   opAt 456 .JUMPDEST,
+   opAt 457 .JUMPDEST,
+   opAt 458 .ISZERO,
+   pushAt 459 2 800,
+   opAt 460 .JUMPI]
 
 end Challenge.Modexp.Submission.Proofs.Fast
