Challenge/Modexp/Submission/Proofs/Fast/ShiftTrace2.lean
@@ -27,206 +27,206 @@ open Challenge.Modexp.Submission.Proofs.Fast
 open Challenge.Modexp.Submission.Proofs.Bytecode
 open Challenge.Modexp.Submission.Proofs.Bytecode.ShiftPCs
 
-@[simp] private theorem followupPC2764 : Artifact.submissionArtifact.instructionPC 2465 = 3054 := by
+@[simp] private theorem followupPC2764 : Artifact.submissionArtifact.instructionPC 2478 = 3054 := by
   rw [Challenge.Modexp.Submission.Proofs.Bytecode.PCFast.instructionPC_eq_byteLength]
   rfl
 
-@[simp] private theorem followupPC2765 : Artifact.submissionArtifact.instructionPC 2466 = 3057 := by
+@[simp] private theorem followupPC2765 : Artifact.submissionArtifact.instructionPC 2479 = 3057 := by
   rw [Challenge.Modexp.Submission.Proofs.Bytecode.PCFast.instructionPC_eq_byteLength]
   rfl
 
-@[simp] private theorem compactLoopPC2749 : Artifact.submissionArtifact.instructionPC 2459 = 3048 := by
+@[simp] private theorem compactLoopPC2749 : Artifact.submissionArtifact.instructionPC 2472 = 3048 := by
   rw [Challenge.Modexp.Submission.Proofs.Bytecode.PCFast.instructionPC_eq_byteLength]
   rfl
 
-@[simp] private theorem compactLoopPC2750 : Artifact.submissionArtifact.instructionPC 2460 = 3049 := by
+@[simp] private theorem compactLoopPC2750 : Artifact.submissionArtifact.instructionPC 2473 = 3049 := by
   rw [Challenge.Modexp.Submission.Proofs.Bytecode.PCFast.instructionPC_eq_byteLength]
   rfl
 
-@[simp] private theorem compactLoopPC2751 : Artifact.submissionArtifact.instructionPC 2461 = 3050 := by
+@[simp] private theorem compactLoopPC2751 : Artifact.submissionArtifact.instructionPC 2474 = 3050 := by
   rw [Challenge.Modexp.Submission.Proofs.Bytecode.PCFast.instructionPC_eq_byteLength]
   rfl
 
-@[simp] private theorem compactLoopPC2752 : Artifact.submissionArtifact.instructionPC 2464 = 3053 := by
+@[simp] private theorem compactLoopPC2752 : Artifact.submissionArtifact.instructionPC 2477 = 3053 := by
   rw [Challenge.Modexp.Submission.Proofs.Bytecode.PCFast.instructionPC_eq_byteLength]
   rfl
 
-@[simp] private theorem compactLoopPC2753 : Artifact.submissionArtifact.instructionPC 2464 = 3053 := by
+@[simp] private theorem compactLoopPC2753 : Artifact.submissionArtifact.instructionPC 2477 = 3053 := by
   rw [Challenge.Modexp.Submission.Proofs.Bytecode.PCFast.instructionPC_eq_byteLength]
   rfl
 
-@[simp] private theorem compactLoopPC2754 : Artifact.submissionArtifact.instructionPC 2464 = 3053 := by
+@[simp] private theorem compactLoopPC2754 : Artifact.submissionArtifact.instructionPC 2477 = 3053 := by
   rw [Challenge.Modexp.Submission.Proofs.Bytecode.PCFast.instructionPC_eq_byteLength]
   rfl
 
-@[simp] private theorem compactLoopPC2755 : Artifact.submissionArtifact.instructionPC 2464 = 3053 := by
-  rw [Challenge.Modexp.Submission.Proofs.Bytecode.PCFast.instructionPC_eq_byteLength]
-  rfl
-
-
-@[simp] private theorem compactLoopPC2758 : Artifact.submissionArtifact.instructionPC 2467 = 3058 := by
-  rw [Challenge.Modexp.Submission.Proofs.Bytecode.PCFast.instructionPC_eq_byteLength]
-  rfl
-
-@[simp] private theorem compactLoopPC2759 : Artifact.submissionArtifact.instructionPC 2468 = 3059 := by
-  rw [Challenge.Modexp.Submission.Proofs.Bytecode.PCFast.instructionPC_eq_byteLength]
-  rfl
-
-@[simp] private theorem compactLoopPC2760 : Artifact.submissionArtifact.instructionPC 2468 = 3059 := by
-  rw [Challenge.Modexp.Submission.Proofs.Bytecode.PCFast.instructionPC_eq_byteLength]
-  rfl
-
-@[simp] private theorem compactLoopPC2761 : Artifact.submissionArtifact.instructionPC 2468 = 3059 := by
+@[simp] private theorem compactLoopPC2755 : Artifact.submissionArtifact.instructionPC 2477 = 3053 := by
   rw [Challenge.Modexp.Submission.Proofs.Bytecode.PCFast.instructionPC_eq_byteLength]
   rfl
 
 
-
-@[simp] private theorem compactLoopPC2764 : Artifact.submissionArtifact.instructionPC 2471 = 3062 := by
+@[simp] private theorem compactLoopPC2758 : Artifact.submissionArtifact.instructionPC 2480 = 3058 := by
   rw [Challenge.Modexp.Submission.Proofs.Bytecode.PCFast.instructionPC_eq_byteLength]
   rfl
 
-@[simp] private theorem compactLoopPC2765 : Artifact.submissionArtifact.instructionPC 2472 = 3063 := by
+@[simp] private theorem compactLoopPC2759 : Artifact.submissionArtifact.instructionPC 2481 = 3059 := by
   rw [Challenge.Modexp.Submission.Proofs.Bytecode.PCFast.instructionPC_eq_byteLength]
   rfl
 
-@[simp] private theorem compactLoopPC2766 : Artifact.submissionArtifact.instructionPC 2473 = 3064 := by
+@[simp] private theorem compactLoopPC2760 : Artifact.submissionArtifact.instructionPC 2481 = 3059 := by
   rw [Challenge.Modexp.Submission.Proofs.Bytecode.PCFast.instructionPC_eq_byteLength]
   rfl
 
-@[simp] private theorem compactLoopPC2767 : Artifact.submissionArtifact.instructionPC 2474 = 3065 := by
+@[simp] private theorem compactLoopPC2761 : Artifact.submissionArtifact.instructionPC 2481 = 3059 := by
   rw [Challenge.Modexp.Submission.Proofs.Bytecode.PCFast.instructionPC_eq_byteLength]
   rfl
 
-@[simp] private theorem compactLoopPC2768 : Artifact.submissionArtifact.instructionPC 2475 = 3066 := by
+
+
+@[simp] private theorem compactLoopPC2764 : Artifact.submissionArtifact.instructionPC 2484 = 3062 := by
   rw [Challenge.Modexp.Submission.Proofs.Bytecode.PCFast.instructionPC_eq_byteLength]
   rfl
 
-@[simp] private theorem compactLoopPC2769 : Artifact.submissionArtifact.instructionPC 2476 = 3067 := by
+@[simp] private theorem compactLoopPC2765 : Artifact.submissionArtifact.instructionPC 2485 = 3063 := by
   rw [Challenge.Modexp.Submission.Proofs.Bytecode.PCFast.instructionPC_eq_byteLength]
   rfl
 
-@[simp] private theorem compactLoopPC2770 : Artifact.submissionArtifact.instructionPC 2477 = 3068 := by
+@[simp] private theorem compactLoopPC2766 : Artifact.submissionArtifact.instructionPC 2486 = 3064 := by
   rw [Challenge.Modexp.Submission.Proofs.Bytecode.PCFast.instructionPC_eq_byteLength]
   rfl
 
-@[simp] private theorem compactLoopPC2771 : Artifact.submissionArtifact.instructionPC 2478 = 3069 := by
+@[simp] private theorem compactLoopPC2767 : Artifact.submissionArtifact.instructionPC 2487 = 3065 := by
   rw [Challenge.Modexp.Submission.Proofs.Bytecode.PCFast.instructionPC_eq_byteLength]
   rfl
 
-@[simp] private theorem compactLoopPC2772 : Artifact.submissionArtifact.instructionPC 2479 = 3070 := by
+@[simp] private theorem compactLoopPC2768 : Artifact.submissionArtifact.instructionPC 2488 = 3066 := by
   rw [Challenge.Modexp.Submission.Proofs.Bytecode.PCFast.instructionPC_eq_byteLength]
   rfl
 
-@[simp] private theorem compactLoopPC2773 : Artifact.submissionArtifact.instructionPC 2480 = 3071 := by
+@[simp] private theorem compactLoopPC2769 : Artifact.submissionArtifact.instructionPC 2489 = 3067 := by
   rw [Challenge.Modexp.Submission.Proofs.Bytecode.PCFast.instructionPC_eq_byteLength]
   rfl
 
-@[simp] private theorem compactLoopPC2774 : Artifact.submissionArtifact.instructionPC 2481 = 3072 := by
+@[simp] private theorem compactLoopPC2770 : Artifact.submissionArtifact.instructionPC 2490 = 3068 := by
   rw [Challenge.Modexp.Submission.Proofs.Bytecode.PCFast.instructionPC_eq_byteLength]
   rfl
 
-@[simp] private theorem compactLoopPC2775 : Artifact.submissionArtifact.instructionPC 2482 = 3075 := by
+@[simp] private theorem compactLoopPC2771 : Artifact.submissionArtifact.instructionPC 2491 = 3069 := by
   rw [Challenge.Modexp.Submission.Proofs.Bytecode.PCFast.instructionPC_eq_byteLength]
   rfl
 
-@[simp] private theorem compactLoopPC2776 : Artifact.submissionArtifact.instructionPC 2483 = 3076 := by
+@[simp] private theorem compactLoopPC2772 : Artifact.submissionArtifact.instructionPC 2492 = 3070 := by
   rw [Challenge.Modexp.Submission.Proofs.Bytecode.PCFast.instructionPC_eq_byteLength]
   rfl
 
-@[simp] private theorem compactLoopPC2777 : Artifact.submissionArtifact.instructionPC 2484 = 3077 := by
+@[simp] private theorem compactLoopPC2773 : Artifact.submissionArtifact.instructionPC 2493 = 3071 := by
   rw [Challenge.Modexp.Submission.Proofs.Bytecode.PCFast.instructionPC_eq_byteLength]
   rfl
 
-@[simp] private theorem compactLoopPC2778 : Artifact.submissionArtifact.instructionPC 2485 = 3078 := by
+@[simp] private theorem compactLoopPC2774 : Artifact.submissionArtifact.instructionPC 2494 = 3072 := by
   rw [Challenge.Modexp.Submission.Proofs.Bytecode.PCFast.instructionPC_eq_byteLength]
   rfl
 
-@[simp] private theorem compactLoopPC2779 : Artifact.submissionArtifact.instructionPC 2486 = 3079 := by
+@[simp] private theorem compactLoopPC2775 : Artifact.submissionArtifact.instructionPC 2495 = 3075 := by
   rw [Challenge.Modexp.Submission.Proofs.Bytecode.PCFast.instructionPC_eq_byteLength]
   rfl
 
-@[simp] private theorem compactLoopPC2780 : Artifact.submissionArtifact.instructionPC 2487 = 3082 := by
+@[simp] private theorem compactLoopPC2776 : Artifact.submissionArtifact.instructionPC 2496 = 3076 := by
   rw [Challenge.Modexp.Submission.Proofs.Bytecode.PCFast.instructionPC_eq_byteLength]
   rfl
 
-@[simp] private theorem compactLoopPC2781 : Artifact.submissionArtifact.instructionPC 2488 = 3083 := by
+@[simp] private theorem compactLoopPC2777 : Artifact.submissionArtifact.instructionPC 2497 = 3077 := by
   rw [Challenge.Modexp.Submission.Proofs.Bytecode.PCFast.instructionPC_eq_byteLength]
   rfl
 
-@[simp] private theorem compactLoopPC2782 : Artifact.submissionArtifact.instructionPC 2489 = 3084 := by
+@[simp] private theorem compactLoopPC2778 : Artifact.submissionArtifact.instructionPC 2498 = 3078 := by
   rw [Challenge.Modexp.Submission.Proofs.Bytecode.PCFast.instructionPC_eq_byteLength]
   rfl
 
-@[simp] private theorem compactLoopPC2783 : Artifact.submissionArtifact.instructionPC 2490 = 3085 := by
+@[simp] private theorem compactLoopPC2779 : Artifact.submissionArtifact.instructionPC 2499 = 3079 := by
   rw [Challenge.Modexp.Submission.Proofs.Bytecode.PCFast.instructionPC_eq_byteLength]
   rfl
 
-@[simp] private theorem compactLoopPC2784 : Artifact.submissionArtifact.instructionPC 2491 = 3086 := by
+@[simp] private theorem compactLoopPC2780 : Artifact.submissionArtifact.instructionPC 2500 = 3082 := by
   rw [Challenge.Modexp.Submission.Proofs.Bytecode.PCFast.instructionPC_eq_byteLength]
   rfl
 
-@[simp] private theorem compactLoopPC2785 : Artifact.submissionArtifact.instructionPC 2492 = 3087 := by
+@[simp] private theorem compactLoopPC2781 : Artifact.submissionArtifact.instructionPC 2501 = 3083 := by
   rw [Challenge.Modexp.Submission.Proofs.Bytecode.PCFast.instructionPC_eq_byteLength]
   rfl
 
-@[simp] private theorem compactLoopPC2786 : Artifact.submissionArtifact.instructionPC 2493 = 3088 := by
+@[simp] private theorem compactLoopPC2782 : Artifact.submissionArtifact.instructionPC 2502 = 3084 := by
   rw [Challenge.Modexp.Submission.Proofs.Bytecode.PCFast.instructionPC_eq_byteLength]
   rfl
 
-@[simp] private theorem compactLoopPC2787 : Artifact.submissionArtifact.instructionPC 2494 = 3089 := by
+@[simp] private theorem compactLoopPC2783 : Artifact.submissionArtifact.instructionPC 2503 = 3085 := by
   rw [Challenge.Modexp.Submission.Proofs.Bytecode.PCFast.instructionPC_eq_byteLength]
   rfl
 
-@[simp] private theorem compactLoopPC2788 : Artifact.submissionArtifact.instructionPC 2495 = 3090 := by
+@[simp] private theorem compactLoopPC2784 : Artifact.submissionArtifact.instructionPC 2504 = 3086 := by
   rw [Challenge.Modexp.Submission.Proofs.Bytecode.PCFast.instructionPC_eq_byteLength]
   rfl
 
-@[simp] private theorem compactLoopPC2789 : Artifact.submissionArtifact.instructionPC 2496 = 3091 := by
+@[simp] private theorem compactLoopPC2785 : Artifact.submissionArtifact.instructionPC 2505 = 3087 := by
   rw [Challenge.Modexp.Submission.Proofs.Bytecode.PCFast.instructionPC_eq_byteLength]
   rfl
 
-@[simp] private theorem compactLoopPC2790 : Artifact.submissionArtifact.instructionPC 2497 = 3092 := by
+@[simp] private theorem compactLoopPC2786 : Artifact.submissionArtifact.instructionPC 2506 = 3088 := by
   rw [Challenge.Modexp.Submission.Proofs.Bytecode.PCFast.instructionPC_eq_byteLength]
   rfl
 
-@[simp] private theorem compactLoopPC2791 : Artifact.submissionArtifact.instructionPC 2498 = 3093 := by
+@[simp] private theorem compactLoopPC2787 : Artifact.submissionArtifact.instructionPC 2507 = 3089 := by
   rw [Challenge.Modexp.Submission.Proofs.Bytecode.PCFast.instructionPC_eq_byteLength]
   rfl
 
-@[simp] private theorem compactLoopPC2792 : Artifact.submissionArtifact.instructionPC 2499 = 3096 := by
+@[simp] private theorem compactLoopPC2788 : Artifact.submissionArtifact.instructionPC 2508 = 3090 := by
   rw [Challenge.Modexp.Submission.Proofs.Bytecode.PCFast.instructionPC_eq_byteLength]
   rfl
 
-@[simp] private theorem compactLoopPC2793 : Artifact.submissionArtifact.instructionPC 2500 = 3097 := by
+@[simp] private theorem compactLoopPC2789 : Artifact.submissionArtifact.instructionPC 2509 = 3091 := by
   rw [Challenge.Modexp.Submission.Proofs.Bytecode.PCFast.instructionPC_eq_byteLength]
   rfl
 
-@[simp] private theorem compactLoopPC2794 : Artifact.submissionArtifact.instructionPC 2501 = 3098 := by
+@[simp] private theorem compactLoopPC2790 : Artifact.submissionArtifact.instructionPC 2510 = 3092 := by
   rw [Challenge.Modexp.Submission.Proofs.Bytecode.PCFast.instructionPC_eq_byteLength]
   rfl
 
-@[simp] private theorem compactLoopPC2795 : Artifact.submissionArtifact.instructionPC 2502 = 3099 := by
+@[simp] private theorem compactLoopPC2791 : Artifact.submissionArtifact.instructionPC 2511 = 3093 := by
   rw [Challenge.Modexp.Submission.Proofs.Bytecode.PCFast.instructionPC_eq_byteLength]
   rfl
 
-@[simp] private theorem compactLoopPC2797 : Artifact.submissionArtifact.instructionPC 2613 = 3246 := by
+@[simp] private theorem compactLoopPC2792 : Artifact.submissionArtifact.instructionPC 2512 = 3096 := by
   rw [Challenge.Modexp.Submission.Proofs.Bytecode.PCFast.instructionPC_eq_byteLength]
   rfl
 
-@[simp] private theorem compactLoopPC2798 : Artifact.submissionArtifact.instructionPC 2614 = 3247 := by
+@[simp] private theorem compactLoopPC2793 : Artifact.submissionArtifact.instructionPC 2513 = 3097 := by
   rw [Challenge.Modexp.Submission.Proofs.Bytecode.PCFast.instructionPC_eq_byteLength]
   rfl
 
-@[simp] private theorem compactLoopPC2799 : Artifact.submissionArtifact.instructionPC 2615 = 3249 := by
+@[simp] private theorem compactLoopPC2794 : Artifact.submissionArtifact.instructionPC 2514 = 3098 := by
   rw [Challenge.Modexp.Submission.Proofs.Bytecode.PCFast.instructionPC_eq_byteLength]
   rfl
 
-@[simp] private theorem compactLoopPC2800 : Artifact.submissionArtifact.instructionPC 2616 = 3250 := by
+@[simp] private theorem compactLoopPC2795 : Artifact.submissionArtifact.instructionPC 2515 = 3099 := by
   rw [Challenge.Modexp.Submission.Proofs.Bytecode.PCFast.instructionPC_eq_byteLength]
   rfl
 
-@[simp] private theorem compactLoopPC2803 : Artifact.submissionArtifact.instructionPC 2619 = 3255 := by
+@[simp] private theorem compactLoopPC2797 : Artifact.submissionArtifact.instructionPC 2626 = 3246 := by
+  rw [Challenge.Modexp.Submission.Proofs.Bytecode.PCFast.instructionPC_eq_byteLength]
+  rfl
+
+@[simp] private theorem compactLoopPC2798 : Artifact.submissionArtifact.instructionPC 2627 = 3247 := by
+  rw [Challenge.Modexp.Submission.Proofs.Bytecode.PCFast.instructionPC_eq_byteLength]
+  rfl
+
+@[simp] private theorem compactLoopPC2799 : Artifact.submissionArtifact.instructionPC 2628 = 3249 := by
+  rw [Challenge.Modexp.Submission.Proofs.Bytecode.PCFast.instructionPC_eq_byteLength]
+  rfl
+
+@[simp] private theorem compactLoopPC2800 : Artifact.submissionArtifact.instructionPC 2629 = 3250 := by
+  rw [Challenge.Modexp.Submission.Proofs.Bytecode.PCFast.instructionPC_eq_byteLength]
+  rfl
+
+@[simp] private theorem compactLoopPC2803 : Artifact.submissionArtifact.instructionPC 2632 = 3255 := by
   rw [Challenge.Modexp.Submission.Proofs.Bytecode.PCFast.instructionPC_eq_byteLength]
   rfl
 
@@ -328,343 +328,343 @@ private theorem addMod_comm (a b m : UInt256) :
     UInt256.addMod a b m = UInt256.addMod b a m := by
   simp only [UInt256.addMod, Nat.add_comm]
 
-@[simp] private theorem newEstimatePC2960 : Artifact.submissionArtifact.instructionPC 2225 = 2761 := by
+@[simp] private theorem newEstimatePC2960 : Artifact.submissionArtifact.instructionPC 2238 = 2761 := by
   rw [Challenge.Modexp.Submission.Proofs.Bytecode.PCFast.instructionPC_eq_byteLength]
   rfl
 
-@[simp] private theorem newEstimatePC2961 : Artifact.submissionArtifact.instructionPC 2226 = 2762 := by
+@[simp] private theorem newEstimatePC2961 : Artifact.submissionArtifact.instructionPC 2239 = 2762 := by
   rw [Challenge.Modexp.Submission.Proofs.Bytecode.PCFast.instructionPC_eq_byteLength]
   rfl
 
-@[simp] private theorem newEstimatePC2962 : Artifact.submissionArtifact.instructionPC 2227 = 2765 := by
+@[simp] private theorem newEstimatePC2962 : Artifact.submissionArtifact.instructionPC 2240 = 2765 := by
   rw [Challenge.Modexp.Submission.Proofs.Bytecode.PCFast.instructionPC_eq_byteLength]
   rfl
 
-@[simp] private theorem newEstimatePC2963 : Artifact.submissionArtifact.instructionPC 2228 = 2766 := by
+@[simp] private theorem newEstimatePC2963 : Artifact.submissionArtifact.instructionPC 2241 = 2766 := by
   rw [Challenge.Modexp.Submission.Proofs.Bytecode.PCFast.instructionPC_eq_byteLength]
   rfl
 
-@[simp] private theorem newEstimatePC2964 : Artifact.submissionArtifact.instructionPC 2229 = 2767 := by
+@[simp] private theorem newEstimatePC2964 : Artifact.submissionArtifact.instructionPC 2242 = 2767 := by
   rw [Challenge.Modexp.Submission.Proofs.Bytecode.PCFast.instructionPC_eq_byteLength]
   rfl
 
-@[simp] private theorem newEstimatePC2965 : Artifact.submissionArtifact.instructionPC 2230 = 2769 := by
+@[simp] private theorem newEstimatePC2965 : Artifact.submissionArtifact.instructionPC 2243 = 2769 := by
   rw [Challenge.Modexp.Submission.Proofs.Bytecode.PCFast.instructionPC_eq_byteLength]
   rfl
 
-@[simp] private theorem newEstimatePC2966 : Artifact.submissionArtifact.instructionPC 2231 = 2770 := by
+@[simp] private theorem newEstimatePC2966 : Artifact.submissionArtifact.instructionPC 2244 = 2770 := by
   rw [Challenge.Modexp.Submission.Proofs.Bytecode.PCFast.instructionPC_eq_byteLength]
   rfl
 
-@[simp] private theorem newEstimatePC2967 : Artifact.submissionArtifact.instructionPC 2232 = 2772 := by
+@[simp] private theorem newEstimatePC2967 : Artifact.submissionArtifact.instructionPC 2245 = 2772 := by
   rw [Challenge.Modexp.Submission.Proofs.Bytecode.PCFast.instructionPC_eq_byteLength]
   rfl
 
-@[simp] private theorem newEstimatePCk2750 : Artifact.submissionArtifact.instructionPC 2233 = 2773 := by
+@[simp] private theorem newEstimatePCk2750 : Artifact.submissionArtifact.instructionPC 2246 = 2773 := by
   rw [Challenge.Modexp.Submission.Proofs.Bytecode.PCFast.instructionPC_eq_byteLength]
   rfl
 
-@[simp] private theorem newEstimatePCk2751 : Artifact.submissionArtifact.instructionPC 2234 = 2774 := by
+@[simp] private theorem newEstimatePCk2751 : Artifact.submissionArtifact.instructionPC 2247 = 2774 := by
   rw [Challenge.Modexp.Submission.Proofs.Bytecode.PCFast.instructionPC_eq_byteLength]
   rfl
 
-@[simp] private theorem newEstimatePCk2752 : Artifact.submissionArtifact.instructionPC 2235 = 2776 := by
+@[simp] private theorem newEstimatePCk2752 : Artifact.submissionArtifact.instructionPC 2248 = 2776 := by
   rw [Challenge.Modexp.Submission.Proofs.Bytecode.PCFast.instructionPC_eq_byteLength]
   rfl
 
-@[simp] private theorem newEstimatePCk2753 : Artifact.submissionArtifact.instructionPC 2236 = 2777 := by
+@[simp] private theorem newEstimatePCk2753 : Artifact.submissionArtifact.instructionPC 2249 = 2777 := by
   rw [Challenge.Modexp.Submission.Proofs.Bytecode.PCFast.instructionPC_eq_byteLength]
   rfl
 
-@[simp] private theorem newEstimatePCk2754 : Artifact.submissionArtifact.instructionPC 2237 = 2778 := by
+@[simp] private theorem newEstimatePCk2754 : Artifact.submissionArtifact.instructionPC 2250 = 2778 := by
   rw [Challenge.Modexp.Submission.Proofs.Bytecode.PCFast.instructionPC_eq_byteLength]
   rfl
 
-@[simp] private theorem newEstimatePCk2755 : Artifact.submissionArtifact.instructionPC 2238 = 2779 := by
+@[simp] private theorem newEstimatePCk2755 : Artifact.submissionArtifact.instructionPC 2251 = 2779 := by
   rw [Challenge.Modexp.Submission.Proofs.Bytecode.PCFast.instructionPC_eq_byteLength]
   rfl
 
-@[simp] private theorem newEstimatePCk2756 : Artifact.submissionArtifact.instructionPC 2239 = 2780 := by
+@[simp] private theorem newEstimatePCk2756 : Artifact.submissionArtifact.instructionPC 2252 = 2780 := by
   rw [Challenge.Modexp.Submission.Proofs.Bytecode.PCFast.instructionPC_eq_byteLength]
   rfl
 
-@[simp] private theorem newEstimatePCk2757 : Artifact.submissionArtifact.instructionPC 2240 = 2781 := by
+@[simp] private theorem newEstimatePCk2757 : Artifact.submissionArtifact.instructionPC 2253 = 2781 := by
   rw [Challenge.Modexp.Submission.Proofs.Bytecode.PCFast.instructionPC_eq_byteLength]
   rfl
 
-@[simp] private theorem newEstimatePCk2758 : Artifact.submissionArtifact.instructionPC 2241 = 2782 := by
+@[simp] private theorem newEstimatePCk2758 : Artifact.submissionArtifact.instructionPC 2254 = 2782 := by
   rw [Challenge.Modexp.Submission.Proofs.Bytecode.PCFast.instructionPC_eq_byteLength]
   rfl
 
-@[simp] private theorem dagInstructionPC2284 : Artifact.submissionArtifact.instructionPC 2204 = 2732 := by
+@[simp] private theorem dagInstructionPC2284 : Artifact.submissionArtifact.instructionPC 2217 = 2732 := by
   rw [Challenge.Modexp.Submission.Proofs.Bytecode.PCFast.instructionPC_eq_byteLength]
   rfl
 
-@[simp] private theorem dagInstructionPC2285 : Artifact.submissionArtifact.instructionPC 2205 = 2735 := by
+@[simp] private theorem dagInstructionPC2285 : Artifact.submissionArtifact.instructionPC 2218 = 2735 := by
   rw [Challenge.Modexp.Submission.Proofs.Bytecode.PCFast.instructionPC_eq_byteLength]
   rfl
 
-@[simp] private theorem dagInstructionPC2286 : Artifact.submissionArtifact.instructionPC 2206 = 2736 := by
+@[simp] private theorem dagInstructionPC2286 : Artifact.submissionArtifact.instructionPC 2219 = 2736 := by
   rw [Challenge.Modexp.Submission.Proofs.Bytecode.PCFast.instructionPC_eq_byteLength]
   rfl
 
-@[simp] private theorem dagInstructionPC2287 : Artifact.submissionArtifact.instructionPC 2207 = 2737 := by
+@[simp] private theorem dagInstructionPC2287 : Artifact.submissionArtifact.instructionPC 2220 = 2737 := by
   rw [Challenge.Modexp.Submission.Proofs.Bytecode.PCFast.instructionPC_eq_byteLength]
   rfl
 
-@[simp] private theorem dagInstructionPC2288 : Artifact.submissionArtifact.instructionPC 2208 = 2738 := by
+@[simp] private theorem dagInstructionPC2288 : Artifact.submissionArtifact.instructionPC 2221 = 2738 := by
   rw [Challenge.Modexp.Submission.Proofs.Bytecode.PCFast.instructionPC_eq_byteLength]
   rfl
 
-@[simp] private theorem dagInstructionPC2333 : Artifact.submissionArtifact.instructionPC 2461 = 3050 := by
+@[simp] private theorem dagInstructionPC2333 : Artifact.submissionArtifact.instructionPC 2474 = 3050 := by
   rw [Challenge.Modexp.Submission.Proofs.Bytecode.PCFast.instructionPC_eq_byteLength]
   rfl
 
-@[simp] private theorem dagInstructionPC2334 : Artifact.submissionArtifact.instructionPC 2462 = 3051 := by
+@[simp] private theorem dagInstructionPC2334 : Artifact.submissionArtifact.instructionPC 2475 = 3051 := by
   rw [Challenge.Modexp.Submission.Proofs.Bytecode.PCFast.instructionPC_eq_byteLength]
   rfl
 
-@[simp] private theorem dagInstructionPC2335 : Artifact.submissionArtifact.instructionPC 2463 = 3052 := by
+@[simp] private theorem dagInstructionPC2335 : Artifact.submissionArtifact.instructionPC 2476 = 3052 := by
   rw [Challenge.Modexp.Submission.Proofs.Bytecode.PCFast.instructionPC_eq_byteLength]
   rfl
 
-@[simp] private theorem dagInstructionPC2336 : Artifact.submissionArtifact.instructionPC 2464 = 3053 := by
+@[simp] private theorem dagInstructionPC2336 : Artifact.submissionArtifact.instructionPC 2477 = 3053 := by
   rw [Challenge.Modexp.Submission.Proofs.Bytecode.PCFast.instructionPC_eq_byteLength]
   rfl
 
-@[simp] private theorem nopMovePC2279 : Artifact.submissionArtifact.instructionPC 2199 = 2723 := by
+@[simp] private theorem nopMovePC2279 : Artifact.submissionArtifact.instructionPC 2212 = 2723 := by
   rw [Challenge.Modexp.Submission.Proofs.Bytecode.PCFast.instructionPC_eq_byteLength]
   rfl
 
-@[simp] private theorem nopMovePC2280 : Artifact.submissionArtifact.instructionPC 2200 = 2726 := by
+@[simp] private theorem nopMovePC2280 : Artifact.submissionArtifact.instructionPC 2213 = 2726 := by
   rw [Challenge.Modexp.Submission.Proofs.Bytecode.PCFast.instructionPC_eq_byteLength]
   rfl
 
-@[simp] private theorem nopMovePC2281 : Artifact.submissionArtifact.instructionPC 2201 = 2727 := by
+@[simp] private theorem nopMovePC2281 : Artifact.submissionArtifact.instructionPC 2214 = 2727 := by
   rw [Challenge.Modexp.Submission.Proofs.Bytecode.PCFast.instructionPC_eq_byteLength]
   rfl
 
-@[simp] private theorem nopMovePC2282 : Artifact.submissionArtifact.instructionPC 2202 = 2728 := by
+@[simp] private theorem nopMovePC2282 : Artifact.submissionArtifact.instructionPC 2215 = 2728 := by
   rw [Challenge.Modexp.Submission.Proofs.Bytecode.PCFast.instructionPC_eq_byteLength]
   rfl
 
-@[simp] private theorem nopMovePC2283 : Artifact.submissionArtifact.instructionPC 2203 = 2731 := by
+@[simp] private theorem nopMovePC2283 : Artifact.submissionArtifact.instructionPC 2216 = 2731 := by
   rw [Challenge.Modexp.Submission.Proofs.Bytecode.PCFast.instructionPC_eq_byteLength]
   rfl
 
-@[simp] private theorem nopMovePC2284 : Artifact.submissionArtifact.instructionPC 2204 = 2732 := by
+@[simp] private theorem nopMovePC2284 : Artifact.submissionArtifact.instructionPC 2217 = 2732 := by
   rw [Challenge.Modexp.Submission.Proofs.Bytecode.PCFast.instructionPC_eq_byteLength]
   rfl
 
-@[simp] private theorem nopMovePC2285 : Artifact.submissionArtifact.instructionPC 2205 = 2735 := by
+@[simp] private theorem nopMovePC2285 : Artifact.submissionArtifact.instructionPC 2218 = 2735 := by
   rw [Challenge.Modexp.Submission.Proofs.Bytecode.PCFast.instructionPC_eq_byteLength]
   rfl
 
-@[simp] private theorem nopMovePC2286 : Artifact.submissionArtifact.instructionPC 2206 = 2736 := by
+@[simp] private theorem nopMovePC2286 : Artifact.submissionArtifact.instructionPC 2219 = 2736 := by
   rw [Challenge.Modexp.Submission.Proofs.Bytecode.PCFast.instructionPC_eq_byteLength]
   rfl
 
-@[simp] private theorem nopMovePC2287 : Artifact.submissionArtifact.instructionPC 2207 = 2737 := by
+@[simp] private theorem nopMovePC2287 : Artifact.submissionArtifact.instructionPC 2220 = 2737 := by
   rw [Challenge.Modexp.Submission.Proofs.Bytecode.PCFast.instructionPC_eq_byteLength]
   rfl
 
-@[simp] private theorem nopMovePC2288 : Artifact.submissionArtifact.instructionPC 2208 = 2738 := by
+@[simp] private theorem nopMovePC2288 : Artifact.submissionArtifact.instructionPC 2221 = 2738 := by
   rw [Challenge.Modexp.Submission.Proofs.Bytecode.PCFast.instructionPC_eq_byteLength]
   rfl
 
-@[simp] private theorem nopMovePC2289 : Artifact.submissionArtifact.instructionPC 2209 = 2741 := by
+@[simp] private theorem nopMovePC2289 : Artifact.submissionArtifact.instructionPC 2222 = 2741 := by
   rw [Challenge.Modexp.Submission.Proofs.Bytecode.PCFast.instructionPC_eq_byteLength]
   rfl
 
-@[simp] private theorem nopMovePC2290 : Artifact.submissionArtifact.instructionPC 2210 = 2742 := by
+@[simp] private theorem nopMovePC2290 : Artifact.submissionArtifact.instructionPC 2223 = 2742 := by
   rw [Challenge.Modexp.Submission.Proofs.Bytecode.PCFast.instructionPC_eq_byteLength]
   rfl
 
-@[simp] private theorem nopMovePC2291 : Artifact.submissionArtifact.instructionPC 2211 = 2743 := by
+@[simp] private theorem nopMovePC2291 : Artifact.submissionArtifact.instructionPC 2224 = 2743 := by
   rw [Challenge.Modexp.Submission.Proofs.Bytecode.PCFast.instructionPC_eq_byteLength]
   rfl
 
-@[simp] private theorem nopMovePC2292 : Artifact.submissionArtifact.instructionPC 2212 = 2746 := by
+@[simp] private theorem nopMovePC2292 : Artifact.submissionArtifact.instructionPC 2225 = 2746 := by
   rw [Challenge.Modexp.Submission.Proofs.Bytecode.PCFast.instructionPC_eq_byteLength]
   rfl
 
-@[simp] private theorem nopMovePC2293 : Artifact.submissionArtifact.instructionPC 2213 = 2747 := by
+@[simp] private theorem nopMovePC2293 : Artifact.submissionArtifact.instructionPC 2226 = 2747 := by
   rw [Challenge.Modexp.Submission.Proofs.Bytecode.PCFast.instructionPC_eq_byteLength]
   rfl
 
-@[simp] private theorem nopMovePC2294 : Artifact.submissionArtifact.instructionPC 2214 = 2748 := by
+@[simp] private theorem nopMovePC2294 : Artifact.submissionArtifact.instructionPC 2227 = 2748 := by
   rw [Challenge.Modexp.Submission.Proofs.Bytecode.PCFast.instructionPC_eq_byteLength]
   rfl
 
-@[simp] private theorem nopMovePC2295 : Artifact.submissionArtifact.instructionPC 2215 = 2749 := by
+@[simp] private theorem nopMovePC2295 : Artifact.submissionArtifact.instructionPC 2228 = 2749 := by
   rw [Challenge.Modexp.Submission.Proofs.Bytecode.PCFast.instructionPC_eq_byteLength]
   rfl
 
-@[simp] private theorem nopMovePC2296 : Artifact.submissionArtifact.instructionPC 2216 = 2750 := by
+@[simp] private theorem nopMovePC2296 : Artifact.submissionArtifact.instructionPC 2229 = 2750 := by
   rw [Challenge.Modexp.Submission.Proofs.Bytecode.PCFast.instructionPC_eq_byteLength]
   rfl
 
-@[simp] private theorem nopMovePC2297 : Artifact.submissionArtifact.instructionPC 2217 = 2751 := by
+@[simp] private theorem nopMovePC2297 : Artifact.submissionArtifact.instructionPC 2230 = 2751 := by
   rw [Challenge.Modexp.Submission.Proofs.Bytecode.PCFast.instructionPC_eq_byteLength]
   rfl
 
-@[simp] private theorem nopMovePC2298 : Artifact.submissionArtifact.instructionPC 2218 = 2752 := by
+@[simp] private theorem nopMovePC2298 : Artifact.submissionArtifact.instructionPC 2231 = 2752 := by
   rw [Challenge.Modexp.Submission.Proofs.Bytecode.PCFast.instructionPC_eq_byteLength]
   rfl
 
-@[simp] private theorem nopMovePC2299 : Artifact.submissionArtifact.instructionPC 2219 = 2753 := by
+@[simp] private theorem nopMovePC2299 : Artifact.submissionArtifact.instructionPC 2232 = 2753 := by
   rw [Challenge.Modexp.Submission.Proofs.Bytecode.PCFast.instructionPC_eq_byteLength]
   rfl
 
-@[simp] private theorem nopMovePC2300 : Artifact.submissionArtifact.instructionPC 2220 = 2756 := by
+@[simp] private theorem nopMovePC2300 : Artifact.submissionArtifact.instructionPC 2233 = 2756 := by
   rw [Challenge.Modexp.Submission.Proofs.Bytecode.PCFast.instructionPC_eq_byteLength]
   rfl
 
-@[simp] private theorem nopMovePC2301 : Artifact.submissionArtifact.instructionPC 2221 = 2757 := by
+@[simp] private theorem nopMovePC2301 : Artifact.submissionArtifact.instructionPC 2234 = 2757 := by
   rw [Challenge.Modexp.Submission.Proofs.Bytecode.PCFast.instructionPC_eq_byteLength]
   rfl
 
-@[simp] private theorem nopMovePC2302 : Artifact.submissionArtifact.instructionPC 2222 = 2758 := by
+@[simp] private theorem nopMovePC2302 : Artifact.submissionArtifact.instructionPC 2235 = 2758 := by
   rw [Challenge.Modexp.Submission.Proofs.Bytecode.PCFast.instructionPC_eq_byteLength]
   rfl
 
-@[simp] private theorem nopMovePC2303 : Artifact.submissionArtifact.instructionPC 2223 = 2759 := by
+@[simp] private theorem nopMovePC2303 : Artifact.submissionArtifact.instructionPC 2236 = 2759 := by
   rw [Challenge.Modexp.Submission.Proofs.Bytecode.PCFast.instructionPC_eq_byteLength]
   rfl
 
-@[simp] private theorem nopMovePC2304 : Artifact.submissionArtifact.instructionPC 2224 = 2760 := by
+@[simp] private theorem nopMovePC2304 : Artifact.submissionArtifact.instructionPC 2237 = 2760 := by
   rw [Challenge.Modexp.Submission.Proofs.Bytecode.PCFast.instructionPC_eq_byteLength]
   rfl
 
-@[simp] private theorem nopMovePC2305 : Artifact.submissionArtifact.instructionPC 2225 = 2761 := by
+@[simp] private theorem nopMovePC2305 : Artifact.submissionArtifact.instructionPC 2238 = 2761 := by
   rw [Challenge.Modexp.Submission.Proofs.Bytecode.PCFast.instructionPC_eq_byteLength]
   rfl
 
-@[simp] private theorem nopMovePC2306 : Artifact.submissionArtifact.instructionPC 2226 = 2762 := by
+@[simp] private theorem nopMovePC2306 : Artifact.submissionArtifact.instructionPC 2239 = 2762 := by
   rw [Challenge.Modexp.Submission.Proofs.Bytecode.PCFast.instructionPC_eq_byteLength]
   rfl
 
-@[simp] private theorem nopMovePC2307 : Artifact.submissionArtifact.instructionPC 2227 = 2765 := by
+@[simp] private theorem nopMovePC2307 : Artifact.submissionArtifact.instructionPC 2240 = 2765 := by
   rw [Challenge.Modexp.Submission.Proofs.Bytecode.PCFast.instructionPC_eq_byteLength]
   rfl
 
-@[simp] private theorem nopMovePC2308 : Artifact.submissionArtifact.instructionPC 2228 = 2766 := by
+@[simp] private theorem nopMovePC2308 : Artifact.submissionArtifact.instructionPC 2241 = 2766 := by
   rw [Challenge.Modexp.Submission.Proofs.Bytecode.PCFast.instructionPC_eq_byteLength]
   rfl
 
-@[simp] private theorem nopMovePC2309 : Artifact.submissionArtifact.instructionPC 2229 = 2767 := by
+@[simp] private theorem nopMovePC2309 : Artifact.submissionArtifact.instructionPC 2242 = 2767 := by
   rw [Challenge.Modexp.Submission.Proofs.Bytecode.PCFast.instructionPC_eq_byteLength]
   rfl
 
-@[simp] private theorem nopMovePC2310 : Artifact.submissionArtifact.instructionPC 2230 = 2769 := by
+@[simp] private theorem nopMovePC2310 : Artifact.submissionArtifact.instructionPC 2243 = 2769 := by
   rw [Challenge.Modexp.Submission.Proofs.Bytecode.PCFast.instructionPC_eq_byteLength]
   rfl
 
-@[simp] private theorem nopMovePC2311 : Artifact.submissionArtifact.instructionPC 2231 = 2770 := by
+@[simp] private theorem nopMovePC2311 : Artifact.submissionArtifact.instructionPC 2244 = 2770 := by
   rw [Challenge.Modexp.Submission.Proofs.Bytecode.PCFast.instructionPC_eq_byteLength]
   rfl
 
-@[simp] private theorem nopMovePC2312 : Artifact.submissionArtifact.instructionPC 2232 = 2772 := by
+@[simp] private theorem nopMovePC2312 : Artifact.submissionArtifact.instructionPC 2245 = 2772 := by
   rw [Challenge.Modexp.Submission.Proofs.Bytecode.PCFast.instructionPC_eq_byteLength]
   rfl
 
-@[simp] private theorem nopMovePC2313 : Artifact.submissionArtifact.instructionPC 2233 = 2773 := by
+@[simp] private theorem nopMovePC2313 : Artifact.submissionArtifact.instructionPC 2246 = 2773 := by
   rw [Challenge.Modexp.Submission.Proofs.Bytecode.PCFast.instructionPC_eq_byteLength]
   rfl
 
-@[simp] private theorem nopMovePC2314 : Artifact.submissionArtifact.instructionPC 2234 = 2774 := by
+@[simp] private theorem nopMovePC2314 : Artifact.submissionArtifact.instructionPC 2247 = 2774 := by
   rw [Challenge.Modexp.Submission.Proofs.Bytecode.PCFast.instructionPC_eq_byteLength]
   rfl
 
-@[simp] private theorem nopMovePC2315 : Artifact.submissionArtifact.instructionPC 2235 = 2776 := by
+@[simp] private theorem nopMovePC2315 : Artifact.submissionArtifact.instructionPC 2248 = 2776 := by
   rw [Challenge.Modexp.Submission.Proofs.Bytecode.PCFast.instructionPC_eq_byteLength]
   rfl
 
-@[simp] private theorem nopMovePC2316 : Artifact.submissionArtifact.instructionPC 2236 = 2777 := by
+@[simp] private theorem nopMovePC2316 : Artifact.submissionArtifact.instructionPC 2249 = 2777 := by
   rw [Challenge.Modexp.Submission.Proofs.Bytecode.PCFast.instructionPC_eq_byteLength]
   rfl
 
-@[simp] private theorem nopMovePC2317 : Artifact.submissionArtifact.instructionPC 2237 = 2778 := by
+@[simp] private theorem nopMovePC2317 : Artifact.submissionArtifact.instructionPC 2250 = 2778 := by
   rw [Challenge.Modexp.Submission.Proofs.Bytecode.PCFast.instructionPC_eq_byteLength]
   rfl
 
-@[simp] private theorem nopMovePC2318 : Artifact.submissionArtifact.instructionPC 2238 = 2779 := by
+@[simp] private theorem nopMovePC2318 : Artifact.submissionArtifact.instructionPC 2251 = 2779 := by
   rw [Challenge.Modexp.Submission.Proofs.Bytecode.PCFast.instructionPC_eq_byteLength]
   rfl
 
-@[simp] private theorem nopMovePC2319 : Artifact.submissionArtifact.instructionPC 2239 = 2780 := by
+@[simp] private theorem nopMovePC2319 : Artifact.submissionArtifact.instructionPC 2252 = 2780 := by
   rw [Challenge.Modexp.Submission.Proofs.Bytecode.PCFast.instructionPC_eq_byteLength]
   rfl
 
-@[simp] private theorem nopMovePC2320 : Artifact.submissionArtifact.instructionPC 2240 = 2781 := by
+@[simp] private theorem nopMovePC2320 : Artifact.submissionArtifact.instructionPC 2253 = 2781 := by
   rw [Challenge.Modexp.Submission.Proofs.Bytecode.PCFast.instructionPC_eq_byteLength]
   rfl
 
-@[simp] private theorem nopMovePC2321 : Artifact.submissionArtifact.instructionPC 2241 = 2782 := by
+@[simp] private theorem nopMovePC2321 : Artifact.submissionArtifact.instructionPC 2254 = 2782 := by
   rw [Challenge.Modexp.Submission.Proofs.Bytecode.PCFast.instructionPC_eq_byteLength]
   rfl
 
-@[simp] private theorem nopMovePC2322 : Artifact.submissionArtifact.instructionPC 2242 = 2785 := by
+@[simp] private theorem nopMovePC2322 : Artifact.submissionArtifact.instructionPC 2255 = 2785 := by
   rw [Challenge.Modexp.Submission.Proofs.Bytecode.PCFast.instructionPC_eq_byteLength]
   rfl
 
-@[simp] private theorem nopMovePC2323 : Artifact.submissionArtifact.instructionPC 2243 = 2786 := by
+@[simp] private theorem nopMovePC2323 : Artifact.submissionArtifact.instructionPC 2256 = 2786 := by
   rw [Challenge.Modexp.Submission.Proofs.Bytecode.PCFast.instructionPC_eq_byteLength]
   rfl
 
-@[simp] private theorem nopMovePC2324 : Artifact.submissionArtifact.instructionPC 2244 = 2787 := by
+@[simp] private theorem nopMovePC2324 : Artifact.submissionArtifact.instructionPC 2257 = 2787 := by
   rw [Challenge.Modexp.Submission.Proofs.Bytecode.PCFast.instructionPC_eq_byteLength]
   rfl
 
-@[simp] private theorem nopMovePC2325 : Artifact.submissionArtifact.instructionPC 2245 = 2788 := by
+@[simp] private theorem nopMovePC2325 : Artifact.submissionArtifact.instructionPC 2258 = 2788 := by
   rw [Challenge.Modexp.Submission.Proofs.Bytecode.PCFast.instructionPC_eq_byteLength]
   rfl
 
-@[simp] private theorem nopMovePC2326 : Artifact.submissionArtifact.instructionPC 2246 = 2789 := by
+@[simp] private theorem nopMovePC2326 : Artifact.submissionArtifact.instructionPC 2259 = 2789 := by
   rw [Challenge.Modexp.Submission.Proofs.Bytecode.PCFast.instructionPC_eq_byteLength]
   rfl
 
-@[simp] private theorem nopMovePC2327 : Artifact.submissionArtifact.instructionPC 2247 = 2790 := by
+@[simp] private theorem nopMovePC2327 : Artifact.submissionArtifact.instructionPC 2260 = 2790 := by
   rw [Challenge.Modexp.Submission.Proofs.Bytecode.PCFast.instructionPC_eq_byteLength]
   rfl
 
-@[simp] private theorem nopMovePC2328 : Artifact.submissionArtifact.instructionPC 2456 = 3043 := by
+@[simp] private theorem nopMovePC2328 : Artifact.submissionArtifact.instructionPC 2469 = 3043 := by
   rw [Challenge.Modexp.Submission.Proofs.Bytecode.PCFast.instructionPC_eq_byteLength]
   rfl
 
-@[simp] private theorem nopMovePC2329 : Artifact.submissionArtifact.instructionPC 2457 = 3046 := by
+@[simp] private theorem nopMovePC2329 : Artifact.submissionArtifact.instructionPC 2470 = 3046 := by
   rw [Challenge.Modexp.Submission.Proofs.Bytecode.PCFast.instructionPC_eq_byteLength]
   rfl
 
-@[simp] private theorem nopMovePC2330 : Artifact.submissionArtifact.instructionPC 2458 = 3047 := by
+@[simp] private theorem nopMovePC2330 : Artifact.submissionArtifact.instructionPC 2471 = 3047 := by
   rw [Challenge.Modexp.Submission.Proofs.Bytecode.PCFast.instructionPC_eq_byteLength]
   rfl
 
-@[simp] private theorem nopMovePC2331 : Artifact.submissionArtifact.instructionPC 2459 = 3048 := by
+@[simp] private theorem nopMovePC2331 : Artifact.submissionArtifact.instructionPC 2472 = 3048 := by
   rw [Challenge.Modexp.Submission.Proofs.Bytecode.PCFast.instructionPC_eq_byteLength]
   rfl
 
-@[simp] private theorem nopMovePC2332 : Artifact.submissionArtifact.instructionPC 2460 = 3049 := by
+@[simp] private theorem nopMovePC2332 : Artifact.submissionArtifact.instructionPC 2473 = 3049 := by
   rw [Challenge.Modexp.Submission.Proofs.Bytecode.PCFast.instructionPC_eq_byteLength]
   rfl
 
-@[simp] private theorem nopMovePC2333 : Artifact.submissionArtifact.instructionPC 2461 = 3050 := by
+@[simp] private theorem nopMovePC2333 : Artifact.submissionArtifact.instructionPC 2474 = 3050 := by
   rw [Challenge.Modexp.Submission.Proofs.Bytecode.PCFast.instructionPC_eq_byteLength]
   rfl
 
-@[simp] private theorem nopMovePC2334 : Artifact.submissionArtifact.instructionPC 2462 = 3051 := by
+@[simp] private theorem nopMovePC2334 : Artifact.submissionArtifact.instructionPC 2475 = 3051 := by
   rw [Challenge.Modexp.Submission.Proofs.Bytecode.PCFast.instructionPC_eq_byteLength]
   rfl
 
-@[simp] private theorem nopMovePC2335 : Artifact.submissionArtifact.instructionPC 2463 = 3052 := by
+@[simp] private theorem nopMovePC2335 : Artifact.submissionArtifact.instructionPC 2476 = 3052 := by
   rw [Challenge.Modexp.Submission.Proofs.Bytecode.PCFast.instructionPC_eq_byteLength]
   rfl
 
-@[simp] private theorem nopMovePC2336 : Artifact.submissionArtifact.instructionPC 2464 = 3053 := by
+@[simp] private theorem nopMovePC2336 : Artifact.submissionArtifact.instructionPC 2477 = 3053 := by
   rw [Challenge.Modexp.Submission.Proofs.Bytecode.PCFast.instructionPC_eq_byteLength]
   rfl
 
-@[simp] private theorem nopMovePC2337 : Artifact.submissionArtifact.instructionPC 2465 = 3054 := by
+@[simp] private theorem nopMovePC2337 : Artifact.submissionArtifact.instructionPC 2478 = 3054 := by
   rw [Challenge.Modexp.Submission.Proofs.Bytecode.PCFast.instructionPC_eq_byteLength]
   rfl
 
